CpcMicro/Proofs/Unproven.lean
@@ -1,0 +1,19 @@
+import CpcMicro.Spec
+
+open Eo
+open Smtm
+
+set_option linter.unusedVariables false
+set_option maxHeartbeats 10000000
+
+namespace RuleProofs
+
+theorem eo_to_smt_well_typed_and_typeof_implies_smt_type
+    (t T : Term) (s : SmtTerm) :
+  __eo_to_smt t = s ->
+  __smtx_typeof s ≠ SmtType.None ->
+  __eo_typeof t = T ->
+  __smtx_typeof s = __eo_to_smt_type T := by
+  sorry
+
+end RuleProofs
